theories/iris/logrel/instr/kinding.v
@@ -48,6 +48,29 @@ Section kinding.
     by inversion H2.
   Qed.
 
+  Lemma has_kind_agree F τ κ κ' :
+    has_kind F τ κ →
+    has_kind F τ κ' →
+    κ = κ'.
+  Proof.
+    intros H1 H2.
+    have Hsome := type_kind_has_kind_is_Some _ _ _ H1.
+    destruct Hsome as [κ'' Hκ''].
+    have Hsub1 := type_kind_has_kind_agree _ _ _ _ H1 Hκ''.
+    have Hsub2 := type_kind_has_kind_agree _ _ _ _ H2 Hκ''.
+    by rewrite Hsub2.
+  Qed.
+
+  Lemma has_kind_agree_f F τ ρ ξ σ ξ' :
+    has_kind F τ (VALTYPE ρ ξ) →
+    has_kind F τ (MEMTYPE σ ξ') →
+    False.
+  Proof.
+    intros H1 H2.
+    have H := has_kind_agree _ _ _ _ H1 H2.
+    inversion H.
+  Qed.
+
   Lemma subkind_rep_inv κ κ' :
     subkind_of κ κ' ->
     kind_rep κ = kind_rep κ'.
