theories/iris/logrel/logrel_properties.v
@@ -1,0 +1,1455 @@
+From Stdlib Require Export ZArith.
+
+From stdpp Require Export base list.
+
+Require Export RecordUpdate.RecordUpdate.
+
+From iris.proofmode Require Export base proofmode classes.
+
+From RichWasm.named_props Require Export named_props custom_syntax.
+From RichWasm Require Export layout syntax typing util.
+Require Export RichWasm.wasm.operations.
+From RichWasm.compiler Require Export prelude codegen instruction module.
+From RichWasm.iris Require Export autowp memory logrel util.
+From RichWasm.iris.logrel Require Export util.
+From RichWasm.iris.language Require Export cwp logpred.
+Require Export RichWasm.iris.logrel.instr.kinding.
+
+Set Bullet Behavior "Strict Subproofs".
+Set Default Goal Selector "!".
+
+Section properties.
+
+  Context `{!logrel_na_invs Σ}.
+  Context `{!wasmG Σ}.
+  Context `{!richwasmG Σ}.
+
+  Variable rti : rt_invariant Σ.
+  Variable sr : store_runtime.
+  Variable mr : module_runtime.
+
+  Lemma has_areps_cons_l ιs ι o os:
+    has_areps (ι :: ιs) (SAtoms (o :: os)) ->
+    has_areps ιs (SAtoms os) /\
+    has_arep ι o.
+  Proof.
+    intros H.
+    unfold has_areps in H.
+    destruct H as [os' [Heq HF]].
+    injection Heq as <-.
+    inversion HF as [| ?? ?? Hhead Htail]; subst.
+    split.
+    - unfold has_areps. eauto.
+    - exact Hhead.
+  Qed.
+
+  Lemma has_areps_cons_r ιs ι o os:
+    has_areps ιs (SAtoms os) ->
+    has_arep ι o ->
+    has_areps (ι :: ιs) (SAtoms (o :: os)).
+  Proof.
+    intros Hareps Harep.
+    unfold has_areps.
+    exists (o :: os).
+    split; first done.
+    apply List.Forall2_cons; first done.
+    destruct Hareps as (? & Heq & Hareps).
+    by inversion Heq; subst.
+  Qed.
+
+  Lemma has_areps_cons ιs ι o os:
+    has_areps ιs (SAtoms os) /\
+    has_arep ι o <->
+    has_areps (ι :: ιs) (SAtoms (o :: os)).
+  Proof.
+    split.
+    - intros [? ?]. by apply has_areps_cons_r.
+    - apply has_areps_cons_l.
+  Qed.
+
+  Lemma has_areps_cons_exists ιs o os:
+    has_areps ιs (SAtoms (o :: os)) ->
+    ∃ ι ιs' , ιs = ι :: ιs' /\
+    has_areps ιs' (SAtoms os) /\
+    has_arep ι o.
+  Proof.
+    intros H.
+    destruct ιs as [| ι ιs'].
+    - destruct H as [os' [Heq HF]].
+      inversion Heq; subst.
+      inversion HF.
+    - do 2 eexists.
+      split; first done.
+      by apply has_areps_cons.
+  Qed.
+
+  Lemma has_areps_exists os :
+    ∃ ιs, has_areps ιs (SAtoms os).
+  Proof.
+    induction os as [| o os' IH].
+    - exists []. exists [].
+      done.
+    - destruct IH as [ιs' IH].
+      destruct o; eexists (_ :: ιs'); apply has_areps_cons; split; try done; unfold has_arep.
+      + by instantiate (1 := PtrR).
+      + by instantiate (1 := I32R).
+      + by instantiate (1 := I64R).
+      + by instantiate (1 := F32R).
+      + by instantiate (1 := F64R).
+  Qed.
+
+  Lemma has_areps_app_l ιs1 os1 ιs2 os2 :
+    has_areps ιs1 (SAtoms os1) ->
+    has_areps ιs2 (SAtoms os2) ->
+    has_areps (ιs1 ++ ιs2) (SAtoms $ os1 ++ os2).
+  Proof.
+    intros [os1' [Heq1 Hf1]] [os2' [Heq2 Hf2]].
+    simplify_eq.
+    exists (os1' ++ os2').
+    split.
+    - done.
+    - by apply Forall2_app.
+  Qed.
+
+  Lemma has_areps_app_r_exists ιs1 ιs2 os :
+    has_areps (ιs1 ++ ιs2) (SAtoms os) ->
+    ∃ os1 os2, os = os1 ++ os2 /\
+    has_areps ιs1 (SAtoms os1) /\
+    has_areps ιs2 (SAtoms os2).
+  Proof.
+    intros [os' [Heq Hf]].
+    simplify_eq.
+    apply Forall2_app_inv_l in Hf as [os1 [os2 [Hf1 [Hf2 ->]]]].
+    exists os1, os2.
+    split; [done|].
+    split.
+    - by exists os1.
+    - by exists os2.
+  Qed.
+
+  Lemma has_areps_app_r_length ιs1 os1 ιs2 os2 :
+    length ιs1 = length os1 ->
+    has_areps (ιs1 ++ ιs2) (SAtoms $ os1 ++ os2) ->
+    has_areps ιs1 (SAtoms os1) /\
+    has_areps ιs2 (SAtoms os2).
+  Proof.
+    intros Hlen [os [Heq Hf]].
+    simplify_eq.
+    apply Forall2_app_inv in Hf as [Hf1 Hf2]; [|done].
+    split.
+    - by exists os1.
+    - by exists os2.
+  Qed.
+
+  Lemma has_areps_length ιs os :
+    has_areps ιs (SAtoms os) ->
+    length ιs = length os.
+  Proof.
+    intros [os' [Heq Hf]].
+    simplify_eq.
+    by eapply Forall2_length.
+  Qed.
+
+  Lemma translate_types_comp_interp_length F τs ts se os :
+    sem_env_interp F se ->
+    prelude.translate_types F.(fc_type_vars) τs = Some ts ->
+    values_interp rti sr se τs os -∗
+    ⌜length os = length ts⌝.
+  Proof.
+    intros. iIntros "Hval".
+    cbn.
+  Admitted.
+
+  Lemma values_interp_one_eq se τ os :
+    values_interp rti sr se [τ] os ⊣⊢ value_interp rti sr se τ (SAtoms os).
+  Proof.
+    unfold values_interp.
+    iSplit.
+    - iIntros "(%vss & -> & H)".
+      rewrite big_sepL2_cons_inv_l.
+      iDestruct "H" as "(%vs & %lnil & -> & Hv & Hnils)".
+      rewrite big_sepL2_nil_inv_l.
+      iDestruct "Hnils" as "->".
+      cbn.
+      by rewrite app_nil_r.
+    - iIntros "H".
+      iExists [os].
+      iSplit.
+      + cbn. by rewrite app_nil_r.
+      + iApply big_sepL2_cons.
+        iFrame.
+        by iApply big_sepL2_nil.
+  Qed.
+
+
+  Lemma value_interp_i31 se os :
+    value_interp rti sr se type_i31 (SAtoms os) -∗ ∃ n, ⌜os = [PtrA n]⌝.
+  Proof.
+    iIntros "Hval".
+    iDestruct "Hval" as "(%κ & %Hκ & Rest)".
+    destruct κ; auto.
+    iDestruct "Rest" as "((%Hareps & %Href) & _)".
+    iPureIntro.
+    inversion Hκ; subst; clear Hκ.
+    destruct Hareps as (os' & Htemp & Harep).
+    inversion Htemp; subst os'; clear Htemp.
+    apply Forall2_length in Harep as Hlen.
+    destruct os as [|o [|os]]; try (inversion Hlen).
+    apply Forall2_cons_1 in Harep as [Harep _].
+    cbn in Harep.
+    destruct o; try (inversion Harep).
+    exists p; auto.
+  Qed.
+
+  Lemma value_interp_i32 se os :
+    value_interp rti sr se type_i32 (SAtoms os) -∗ ∃ n, ⌜os = [I32A n]⌝.
+  Proof.
+    iIntros "Hval".
+    iDestruct "Hval" as "(%κ & %Hκ & Rest)".
+    destruct κ; auto.
+    iDestruct "Rest" as "((%Hareps & %Href) & _)".
+    iPureIntro.
+    inversion Hκ; subst; clear Hκ.
+    destruct Hareps as (os' & Htemp & Harep).
+    inversion Htemp; subst os'; clear Htemp.
+    apply Forall2_length in Harep as Hlen.
+    destruct os as [|o [|os]]; try (inversion Hlen).
+    apply Forall2_cons_1 in Harep as [Harep _].
+    cbn in Harep.
+    destruct o; try (inversion Harep).
+    exists n; auto.
+  Qed.
+
+  Lemma value_interp_coderef se os κ ϕ :
+    value_interp rti sr se (CodeRefT κ ϕ) (SAtoms os) -∗ ∃ n, ⌜os = [I32A n]⌝.
+  Proof.
+    iIntros "Hval".
+    iDestruct "Hval" as "(%κ0 & %Hκ & Rest)".
+    destruct κ0; auto; [ | iDestruct "Rest" as "[[[] _] _]"].
+    iDestruct "Rest" as "((%Hareps & %Href) & Oh)".
+    iDestruct "Oh" as "(%i & %i32 & %j & %cl & %nrepr & %nos & what & nstab & nsfun)".
+    inversion nos; subst; clear nos.
+    auto.
+  Qed.
+
+  Lemma values_interp_nil_l se os :
+    values_interp rti sr se [] os -∗ ⌜os = []⌝.
+  Proof.
+    iIntros "Hos".
+    iDestruct "Hos" as "(%oss & -> & Hoss)".
+    by iDestruct (big_sepL2_nil_inv_l with "Hoss") as "->".
+  Qed.
+
+  Lemma values_interp_cons_l se τ τs os :
+    values_interp rti sr se (τ :: τs) os -∗
+    ∃ os1 os2,
+      ⌜os = os1 ++ os2⌝ ∗
+      value_interp rti sr se τ (SAtoms os1) ∗
+      values_interp rti sr se τs os2.
+  Proof.
+    iIntros "Hos".
+    iDestruct "Hos" as "(%oss & -> & Hoss)".
+    iDestruct (big_sepL2_cons_inv_l with "Hoss") as "(%os & %oss' & -> & Hos & Hoss')".
+    iExists os, (concat oss').
+    rewrite concat_cons.
+    by iFrame.
+  Qed.
+
+  Lemma values_interp_app_l se τs1 τs2 os :
+    values_interp rti sr se (τs1 ++ τs2) os -∗
+    ∃ os1 os2,
+      ⌜os = os1 ++ os2⌝ ∗
+      values_interp rti sr se τs1 os1 ∗
+      values_interp rti sr se τs2 os2.
+  Proof.
+  Admitted.
+
+  Lemma result_type_interp_split wl1 wl2 vs_wl :
+    result_type_interp (wl1 ++ wl2) vs_wl ->
+    ∃ vs_wl1 vs_wl2, vs_wl = vs_wl1 ++ vs_wl2 /\
+    result_type_interp wl1 vs_wl1 /\
+    result_type_interp wl2 vs_wl2.
+  Proof.
+    intros H.
+    unfold result_type_interp in H.
+    apply Forall2_app_inv_l in H.
+    destruct H as [vs_wl1 [vs_wl2 [HF1 [HF2 ->]]]].
+    exists vs_wl1, vs_wl2.
+    eauto.
+  Qed.
+
+  Lemma result_type_interp_combine wl1 wl2 vs_wl1 vs_wl2 :
+    result_type_interp wl1 vs_wl1 →
+    result_type_interp wl2 vs_wl2 →
+    result_type_interp (wl1 ++ wl2) (vs_wl1 ++ vs_wl2).
+  Proof.
+    intros H1 H2.
+    unfold result_type_interp in *.
+    apply Forall2_app; eauto.
+  Qed.
+
+  Lemma ref_flag_atoms_interp_cons ξ o os :
+    ref_flag_atoms_interp ξ (SAtoms (o :: os)) ↔
+    forall_ptr_atom (ref_flag_ptr_interp ξ) o ∧ ref_flag_atoms_interp ξ (SAtoms os).
+  Proof.
+    unfold ref_flag_atoms_interp, forall_satoms.
+    by rewrite Forall_cons.
+  Qed.
+
+  Lemma ref_flag_atoms_interp_app ξ os1 os2 :
+    ref_flag_atoms_interp ξ (SAtoms (os1 ++ os2)) ↔
+    ref_flag_atoms_interp ξ (SAtoms os1) ∧ ref_flag_atoms_interp ξ (SAtoms os2).
+  Proof.
+    unfold ref_flag_atoms_interp, forall_satoms.
+    by rewrite Forall_app.
+  Qed.
+
+  Lemma value_interp_ref_flag_atoms se τ ιs ξ sv :
+    type_skind se τ = Some (SVALTYPE ιs ξ) →
+    value_interp rti sr se τ sv -∗
+    ⌜ref_flag_atoms_interp ξ sv⌝.
+  Proof.
+    iIntros (Hskind) "Hval".
+    iDestruct (value_interp_skind with "Hval") as %(sκ & Hsκ & Hsv).
+    rewrite Hskind in Hsκ. inversion Hsκ; subst.
+    iPureIntro.
+    by destruct Hsv.
+  Qed.
+
+  Lemma atoms_interp_nil_l vs :
+    atoms_interp [] vs -∗ ⌜vs = []⌝.
+  Proof.
+    iIntros "Hvs".
+    by iDestruct (big_sepL2_nil_inv_l with "Hvs") as "->".
+  Qed.
+
+  Lemma atoms_interp_cons_l o os vs :
+    atoms_interp (o :: os) vs -∗
+    ∃ v vs',
+      ⌜vs = v :: vs'⌝ ∗
+      atom_interp o v ∗
+      atoms_interp os vs'.
+  Proof.
+    iIntros "Hvs".
+    iDestruct (big_sepL2_cons_inv_l with "Hvs") as "(%v & %vs' & -> & Hv & Hvs')".
+    iExists v, vs'.
+    by iFrame.
+  Qed.
+
+  Lemma atoms_interp_cons o os v vs:
+    atoms_interp (o :: os) (v :: vs) ⊣⊢ atom_interp o v ∗ atoms_interp os vs.
+  Proof.
+    done.
+  Qed.
+
+  Lemma atoms_interp_length os vs :
+    ⊢ atoms_interp os vs -∗ ⌜length os = length vs⌝.
+  Proof.
+    iApply big_sepL2_length.
+  Qed.
+
+  Lemma atoms_interp_one_inv o vs :
+    atoms_interp [o] vs ⊣⊢ ∃ v, ⌜vs = [v]⌝ ∗ atom_interp o v.
+  Proof.
+    iSplit.
+    - iIntros "Hvs".
+      iPoseProof (atoms_interp_cons_l with "Hvs") as (v vs' Heq) "[Hv Hnil]".
+      iPoseProof (atoms_interp_nil_l with "Hnil") as "->".
+      iExists v; auto.
+    - iIntros "(%v & -> & Hv)".
+      cbn; auto.
+  Qed.
+
+  Lemma atom_interp_of_default ty :
+    ⊢ ∃ o, atom_interp o (default_of_value_type ty).
+  Proof.
+    unfold default_of_value_types.
+    destruct ty; iExists _.
+    + instantiate (1 := I32A _); simpl; done.
+    + instantiate (1 := I64A _); simpl; done.
+    + instantiate (1 := F32A _); simpl; done.
+    + instantiate (1 := F64A _); simpl; done.
+  Qed.
+
+  Lemma atoms_interp_of_defaults tys :
+    ⊢ ∃ os, atoms_interp os (default_of_value_types tys).
+  Proof.
+    induction tys as [|ty tys' IH].
+    - iExists [].
+      by simpl.
+    - iDestruct IH as "(%os & IH)".
+      unfold default_of_value_types.
+      rewrite map_cons.
+      iDestruct (atom_interp_of_default ty) as "[%o Hatom]".
+      iExists (o :: os).
+      iApply atoms_interp_cons.
+      by iSplitR.
+  Qed.
+
+  Lemma atom_interp_and_arep_of_default_of_arep ι :
+    ⊢ ∃ o, atom_interp o (default_of_value_type $ translate_arep ι) ∗ ⌜has_arep ι o⌝ ∗ ⌜ref_flag_atoms_interp NoRefs (SAtoms [o])⌝.
+  Proof.
+    destruct ι.
+    - iExists (PtrA _); iSplit; last (iSplit; first done).
+      + simpl.
+        iExists _, _.
+        iSplit; last iSplit; first done.
+        1: done.
+        iExists (RootInt 0).
+        iSplit; first iPureIntro; simpl.
+        1: constructor.
+        by instantiate (1 := PtrInt _).
+      + iPureIntro.
+        unfold ref_flag_atoms_interp, forall_satoms.
+        by apply Forall_singleton.
+    - iExists (I32A _); iSplit; first done.
+      iSplit; first done.
+      iPureIntro.
+      unfold ref_flag_atoms_interp, forall_satoms.
+      by apply Forall_singleton.
+    - iExists (I64A _); iSplit; first done.
+      iSplit; first done.
+      iPureIntro.
+      unfold ref_flag_atoms_interp, forall_satoms.
+      by apply Forall_singleton.
+    - iExists (F32A _); iSplit; first done.
+      iSplit; first done.
+      iPureIntro.
+      unfold ref_flag_atoms_interp, forall_satoms.
+      by apply Forall_singleton.
+    - iExists (F64A _); iSplit; first done.
+      iSplit; first done.
+      iPureIntro.
+      unfold ref_flag_atoms_interp, forall_satoms.
+      by apply Forall_singleton.
+  Qed.
+
+  Lemma atoms_interp_and_areps_of_default_of_areps ιs :
+    ⊢ ∃ os, atoms_interp os (default_of_value_types $ translate_arep <$> ιs) ∗ ⌜has_areps ιs (SAtoms os)⌝ ∗ ⌜ref_flag_atoms_interp NoRefs (SAtoms os)⌝.
+  Proof.
+    induction ιs as [|ι ιs' IH].
+    - iExists [].
+      iSplit; first by simpl.
+      iSplit; first by iExists [].
+      iPureIntro.
+      cbn.
+      done.
+    - iDestruct IH as "(%os' & IHatoms & %IHareps & %IHref_flag)".
+      iEval (unfold default_of_value_types).
+      rewrite fmap_cons.
+      rewrite map_cons.
+      iDestruct (atom_interp_and_arep_of_default_of_arep ι) as "(%o & Hatom & %Harep & %Href_flag)".
+      iExists (o :: os').
+      rewrite atoms_interp_cons.
+      iFrame "#".
+      iPureIntro.
+      split; first by apply has_areps_cons.
+      apply ref_flag_atoms_interp_cons; split; last done.
+      unfold ref_flag_atoms_interp, forall_satoms in Href_flag.
+      by rewrite Forall_singleton in Href_flag.
+  Qed.
+
+    Lemma atoms_interp_take os vs count :
+    atoms_interp os vs -∗
+    atoms_interp (take count os) (take count vs) ∗
+    atoms_interp (drop count os) (drop count vs).
+  Proof.
+    iIntros "Hatoms".
+    iDestruct (big_sepL2_length with "Hatoms") as %Hlen.
+    rewrite -{1}(take_drop count os) -{1}(take_drop count vs).
+    iDestruct (big_sepL2_app_inv with "Hatoms") as "[Htake Hdrop]".
+    { rewrite !length_take. lia. }
+    iFrame.
+  Qed.
+
+  Lemma atoms_interp_take_drop os vs off count :
+    atoms_interp os vs -∗
+    atoms_interp (take count (drop off os)) (take count (drop off vs)).
+  Proof.
+    iIntros "Hatoms".
+    iDestruct (atoms_interp_take with "Hatoms") as "[_ Hdrop]".
+    by iDestruct (atoms_interp_take with "Hdrop") as "[Htake_drop _]".
+  Qed.
+
+  Lemma atoms_interp_app_split_l os1 os2 vs1 vs2 :
+    length os1 = length vs1 ->
+    atoms_interp (os1 ++ os2) (vs1 ++ vs2) -∗
+    atoms_interp os1 vs1 ∗
+    atoms_interp os2 vs2.
+  Proof.
+    iIntros (Hlen) "Hatoms".
+    iDestruct (atoms_interp_take _ _ (length os1) with "Hatoms") as "[H1 H2]".
+    rewrite !take_app_length !drop_app_length Hlen !take_app_length !drop_app_length.
+    iFrame.
+  Qed.
+
+  Lemma atoms_interp_app_split_r os1 os2 vs1 vs2 :
+    atoms_interp os1 vs1 -∗
+    atoms_interp os2 vs2 -∗
+    atoms_interp (os1 ++ os2) (vs1 ++ vs2).
+  Proof.
+    iIntros "H1 H2".
+    iApply (big_sepL2_app with "H1 H2").
+  Qed.
+
+  Lemma atoms_interp_app_l os1 os2 vs :
+    atoms_interp (os1 ++ os2) vs -∗
+    ∃ vs1 vs2, ⌜vs = vs1 ++ vs2⌝ ∗ atoms_interp os1 vs1 ∗ atoms_interp os2 vs2.
+  Proof.
+    iIntros "Hos".
+    iDestruct (atoms_interp_length with "Hos") as %Hlen.
+    iDestruct (atoms_interp_take _ _ (length os1) with "Hos") as "[Hos1 Hos2]".
+    iEval (rewrite take_app_length) in "Hos1".
+    iEval (rewrite drop_app_length) in "Hos2".
+    iExists (take (length os1) vs), (drop (length os1) vs).
+    iSplit.
+    - iPureIntro. rewrite take_drop. reflexivity.
+    - iFrame.
+  Qed.
+
+  Lemma atoms_interp_app_r (os : list atom) (vs1 vs2 : list value) :
+    atoms_interp os (vs1 ++ vs2) -∗
+    ∃ os1 os2 : list atom, ⌜os = os1 ++ os2⌝ ∗ atoms_interp os1 vs1 ∗ atoms_interp os2 vs2.
+  Proof.
+    iIntros "Hos".
+    iDestruct (atoms_interp_length with "Hos") as %Hlen.
+    iDestruct (atoms_interp_take _ _ (length vs1) with "Hos") as "[Hos1 Hos2]".
+    iEval (rewrite take_app_length) in "Hos1".
+    iEval (rewrite drop_app_length) in "Hos2".
+    iExists (take (length vs1) os), (drop (length vs1) os).
+    iSplit.
+    - iPureIntro. rewrite take_drop. reflexivity.
+    - iFrame.
+  Qed.
+
+  Definition value_to_atom (v : value) : atom :=
+    match v with
+    | VAL_int32 n32 => I32A n32
+    | VAL_int64 n64 => I64A n64
+    | VAL_float32 f32 => F32A f32
+    | VAL_float64 f64 => F64A f64
+    end.
+
+  Definition values_to_atoms (vs : list value) :=
+    map value_to_atom vs.
+
+  Lemma atom_interp_value_as_atom v :
+    ⊢ atom_interp (value_to_atom v) v.
+  Proof.
+    destruct v; simpl; by iIntros.
+  Qed.
+
+  Lemma atoms_interp_values_as_atoms vs :
+   ⊢ atoms_interp (values_to_atoms vs) vs.
+  Proof.
+    iInduction vs as [|v vs] "IH"; first by simpl.
+    rewrite /values_to_atoms map_cons.
+    rewrite atoms_interp_cons.
+    iFrame "#".
+    iApply atom_interp_value_as_atom.
+  Qed.
+
+  Definition expect_heap_ptr (o : atom) : option (base_memory * location) :=
+    match o with
+    | PtrA (PtrHeap μ ℓ) => Some (μ, ℓ)
+    | _ => None
+    end.
+
+  Lemma atom_interp_dup o v :
+    expect_heap_ptr o = None ->
+    Persistent (atom_interp o v).
+  Proof.
+    destruct o; cbn; intros Heq; try apply bi.pure_persistent.
+    repeat (apply bi.pure_persistent
+    || (apply bi.exist_persistent; intros ?x)
+    || apply bi.sep_persistent).
+    destruct p; try congruence.
+    destruct x1; cbn;
+    repeat (apply bi.pure_persistent
+    || (apply bi.exist_persistent; intros ?x)
+    || apply bi.sep_persistent).
+  Qed.
+
+  Lemma atoms_interp_dup os vs :
+    Forall (λ o, expect_heap_ptr o = None) os ->
+    Persistent (atoms_interp os vs).
+  Proof.
+    intros Hall.
+    unfold atoms_interp.
+    apply big_sepL2_persistent.
+    intros k o v Hok Hvk.
+    apply atom_interp_dup.
+    rewrite Forall_lookup in Hall.
+    exact (Hall k o Hok).
+  Qed.
+
+  Global Instance atom_interp_value_to_atom_persistent v :
+    Persistent (atom_interp (value_to_atom v) v).
+  Proof.
+    unfold Persistent.
+    iIntros "H !>".
+    iApply atom_interp_value_as_atom.
+  Qed.
+
+  Global Instance atoms_interp_values_to_atoms_persistent vs :
+    Persistent (atoms_interp (values_to_atoms vs) vs).
+  Proof.
+    unfold Persistent.
+    iIntros "H !>".
+    iApply atoms_interp_values_as_atoms.
+  Qed.
+
+  Lemma atoms_interp_norefs_persistent (se: semantic_env (Σ:=Σ)) os vs :
+    ref_flag_atoms_interp NoRefs (SAtoms os) ->
+    Persistent (atoms_interp os vs).
+  Proof.
+    intros Href.
+    unfold ref_flag_atoms_interp, forall_satoms in Href.
+    apply atoms_interp_dup.
+    rewrite Forall_lookup. intros k o Hok.
+    rewrite Forall_lookup in Href.
+    specialize (Href k o Hok).
+    destruct o; simpl in *; try done.
+    destruct p; simpl in *; done.
+  Qed.
+
+
+
+  Lemma frame_interp_wl_interp se F L WL ηss fr :
+    frame_interp rti sr se ηss L WL fr -∗
+    ⌜wl_interp (fe_wlocal_offset (fe_of_context F)) WL fr⌝.
+  Proof.
+    iIntros "Hframe".
+    iDestruct "Hframe" as
+      "(%oss & %vss_L & %vs_WL & %Hfr & %Hprims & %Hresult & Hatom & Hval)".
+    unfold wl_interp.
+
+    (* This is my best guess at the exists given Hfr and Hresult. Should be right *)
+    iExists (concat vss_L). iExists vs_WL. iExists [].
+    iSplit; [|iSplit]; clear_nils; subst; auto.
+
+    iEval (cbn).
+    iEval (cbn) in "Hval".
+    iPoseProof (big_sepL2_length with "[$Hval]") as "%HlenossL".
+    iPoseProof (big_sepL2_length with "[$Hatom]") as "%HlenvssL".
+    rewrite sum_list_with_length_concat.
+    (* unfold atoms_interp; unfold value_interp; destruct F; cbn. *)
+
+    (* Currently unprovable bc there's nothing to relate F fc_locals to *)
+    (* probably need local_ctx_ok F L *)
+
+  Admitted.
+
+    Lemma root_pointer_heap_shp_inv rp μ ℓ :
+    root_pointer_interp rp (PtrHeap μ ℓ) -∗
+    ⌜∃ a, rp = RootHeap μ a⌝.
+  Proof.
+    iIntros "H".
+    destruct rp; first done.
+    cbn.
+    iDestruct "H" as "(-> & _)".
+    by iExists _.
+  Qed.
+
+  Lemma translate_types_sem_interp_length se τs ts os :
+    translate_types se τs = Some ts ->
+    values_interp rti sr se τs os -∗
+    ⌜length os = length ts⌝.
+  Proof.
+    generalize dependent se; generalize dependent ts; generalize dependent os.
+    induction τs.
+    - intros.
+      iIntros  "(%oss & %ossconc & Hval)".
+      iPoseProof (big_sepL2_length with "[$Hval]") as "%osslen".
+      simpl in osslen; destruct oss; [ | inversion osslen].
+      simpl in ossconc; subst; iPureIntro.
+      cbn in H.
+      inversion H; auto.
+    - intros.
+      rewrite separate1.
+      iIntros "Hval".
+      iPoseProof (values_interp_app_l with "[$Hval]") as "(%os1 & %os2 & %Hoslen & Ha & Hτs)".
+      rewrite values_interp_one_eq.
+
+      unfold translate_types in H.
+      rewrite fmap_Some in H.
+      destruct H as (tss & Hmapm & Htsconcat).
+      simpl in Hmapm.
+      apply bind_Some in Hmapm.
+      destruct Hmapm as (ts1 & Htranslate & Hmapτs).
+      set (asdf := translate_types se τs).
+      assert (H: asdf = Some ts). {
+        admit.
+      }
+      (* NOTE: I need to turn Hmapτs back into translate_types se τs = Some _. Or get it out of
+         there at least. Not rn. For now I'll just show stuff about a, aka that os1 = ts1. *)
+
+      subst.
+      (* induction on a? I need to prove that length os1 = length ts1, and that'll
+       depend on what sort of instruction a is. There's some annoying fixpoint here and there. *)
+
+  Admitted.
+
+
+
+
+  Lemma translate_types_comp_sem F τs ts se :
+    sem_env_interp F se ->
+    prelude.translate_types F.(fc_type_vars) τs = Some ts ->
+    @translate_types Σ se τs = Some ts.
+  Admitted.
+
+  Lemma labels_interp_cons se fr wl lmask F L B τs ts Φ :
+    sem_env_interp F se ->
+    prelude.translate_types F.(fc_type_vars) τs = Some ts ->
+    □ (∀ fr' vs',
+       (⌜frame_rel lmask fr fr'⌝ ∗ frame_interp rti sr se F.(typing.fc_locals) L wl fr' ∗
+          (∃ os', values_interp rti sr se τs os' ∗ atoms_interp os' vs') ∗
+          (∃ θ0, rt_token rti sr θ0) ∗ na_own logrel_nais ⊤) -∗
+       Φ fr' vs') -∗
+    labels_interp rti sr se F.(typing.fc_locals) fr wl lmask F.(fc_labels) B -∗
+    labels_interp rti sr se F.(typing.fc_locals) fr wl lmask
+      ((τs, L) :: F.(fc_labels)) ((length ts, Φ) :: B).
+  Proof.
+    iIntros (Hse Hts) "#HΦ Hlabels".
+    unfold labels_interp.
+    unfold const.
+    rewrite big_sepL2_cons.
+    iSplitL "HΦ".
+    - iSplitR.
+      + by erewrite translate_types_comp_sem.
+      + iIntros (fr' vs os θ) "!> %Hlmask Hvs Hos Hown Hframe Hrti".
+        iApply "HΦ".
+        by iFrame.
+    - done.
+  Qed.
+
+
+  Lemma mask_locs_eq_trans lmask fr1 fr2 fr3 :
+    mask_locs_eq lmask fr1 fr2 ->
+    mask_locs_eq lmask fr2 fr3 ->
+    mask_locs_eq lmask fr1 fr3.
+  Proof.
+    intros H12 H23 i Hi.
+    apply H12 in Hi as Hi12.
+    apply H23 in Hi as Hi23.
+    by rewrite Hi12.
+  Qed.
+
+  Lemma frame_rel_trans lmask fr1 fr2 fr3 :
+    frame_rel lmask fr1 fr2 ->
+    frame_rel lmask fr2 fr3 ->
+    frame_rel lmask fr1 fr3.
+  Proof.
+    intros [H12_locs H12_inst] [H23_locs H23_inst].
+    split.
+    - by eapply mask_locs_eq_trans.
+    - by rewrite H12_inst.
+  Qed.
+
+  Lemma labels_interp_trans se wl ηss fr fr' lmask labels B :
+    frame_rel lmask fr fr' ->
+    labels_interp rti sr se ηss fr wl lmask labels B -∗
+    labels_interp rti sr se ηss fr' wl lmask labels B.
+  Proof.
+    iIntros (Heq) "#Hlabels".
+    iApply (big_sepL2_mono with "[$]").
+    iIntros (? [τs L] [n b] Hk_labels Hk_B) "[#Hlen #HP]".
+    iFrame "#".
+    iModIntro.
+    iIntros (?????) "Hframe Hrt Hvs Hos".
+    iApply ("HP" with "[] [$] [$] [$] [$]").
+    iPureIntro.
+    by eapply frame_rel_trans.
+  Qed.
+
+  Lemma frame_rel_mask_mono lmask lmask' fr fr' :
+    (forall i, lmask' i -> lmask i) ->
+    frame_rel lmask fr fr' ->
+    frame_rel lmask' fr fr'.
+  Proof.
+    intros Hmask' [Hmask Hinst].
+    split; last done.
+    intros i Hi.
+    apply Hmask.
+    by apply Hmask'.
+  Qed.
+
+  Lemma frame_rel_wlmask_mono fe wl wl' fr fr' :
+    length wl <= length wl' ->
+    frame_rel (wlmask fe wl') fr fr' ->
+    frame_rel (wlmask fe wl) fr fr'.
+  Proof.
+    intros Hlen Hrel.
+    eapply frame_rel_mask_mono; last done.
+    intros i [Hlo Hhi].
+    split; first done.
+    lia.
+  Qed.
+
+  Lemma labels_interp_mono se ηss fr fr' wl lmask lmask' labels B :
+    frame_rel lmask fr fr' ->
+    (forall i, lmask i -> lmask' i) ->
+    labels_interp rti sr se ηss fr wl lmask labels B -∗
+    labels_interp rti sr se ηss fr' wl lmask' labels B.
+  Proof.
+    iIntros (Hrel Hmask) "#Hlabels".
+    iApply big_sepL2_mono; last done.
+    iIntros (? [τs L] [n b] Hk_labels Hk_B) "[Hlen #HP]".
+    iFrame.
+    iModIntro.
+    iIntros (?????) "Hframe Hrt Hvs Hos".
+    iApply ("HP" with "[] [$] [$] [$] [$]").
+    iPureIntro.
+    eapply frame_rel_trans.
+    - exact Hrel.
+    - by eapply frame_rel_mask_mono.
+  Qed.
+
+  Lemma frame_rel_mask_trans_combine lmask1 lmask2 fr1 fr2 fr3:
+    frame_rel lmask1 fr1 fr2 ->
+    frame_rel lmask2 fr2 fr3 ->
+    frame_rel (λ i, lmask1 i ∧ lmask2 i) fr1 fr3.
+  Proof.
+    intros fr12 fr23.
+    eapply frame_rel_trans;
+      (eapply frame_rel_mask_mono; last done; by intros i [H1 H2]).
+  Qed.
+
+  Lemma frame_f_locs_update fr fr' vs1 vs_new vs_old vs2 val_idxs :
+    val_idxs = seq (length vs1) (length vs_old) ->
+    frame_rel (λ i, i ∉ val_idxs) fr fr' ->
+    Forall2 (λ i v, f_locs fr' !! i = Some v) val_idxs vs_new ->
+    f_locs fr  = vs1 ++ vs_old ++ vs2 ->
+    f_locs fr' = vs1 ++ vs_new ++ vs2.
+  Proof.
+    intros Hval_idxs [Hmask _] HF Hfr.
+    (* First extract length vs_new = length vs_old from Forall2 *)
+    have Hlen : length vs_new = length vs_old.
+    { have := Forall2_length _ _ _ HF. rewrite Hval_idxs length_seq. lia. }
+    (* Prove equality pointwise *)
+    apply list_eq. intros i.
+    destruct (decide (i ∈ val_idxs)) as [Hin | Hout].
+    - (* i is in val_idxs, so fr' !! i = Some (vs_new !! ...) *)
+      rewrite Hval_idxs in Hin.
+      apply elem_of_seq in Hin as [Hlo Hhi].
+      (* j is the position of i in val_idxs *)
+      set j := i - length vs1.
+      have Hj : j < length vs_old by unfold j; lia.
+      have Hseq : seq (length vs1) (length vs_old) !! j = Some i.
+      { rewrite lookup_seq. unfold j. split; lia. }
+      rewrite <- Hval_idxs in Hseq.
+      destruct (Forall2_lookup_l _ _ _ _ _ HF Hseq) as [v [Hv HP]].
+      (* HP : f_locs fr' !! i = Some v *)
+      rewrite HP.
+      (* now show (vs1 ++ vs_new ++ vs2) !! i = Some v *)
+      rewrite lookup_app_r; [|lia].
+      rewrite lookup_app_l; [|rewrite Hlen; lia].
+      (* vs_new !! j = Some v from Hv via HP *)
+      by rewrite Hv.
+    - (* i is not in val_idxs: fr and fr' agree *)
+      rewrite <- Hmask; [|exact Hout].
+      rewrite Hfr.
+      rewrite Hval_idxs in Hout.
+      have Hout' : i < length vs1 ∨ length vs1 + length vs_old ≤ i.
+      { rewrite elem_of_seq in Hout.
+        lia. }
+      destruct Hout' as [Hlt | Hge].
+      + (* i < length vs1: in the vs1 segment, both sides agree *)
+        rewrite !lookup_app_l; lias.
+      + (* i ≥ length vs1 + length vs_old: in the vs2 segment *)
+        rewrite !lookup_app_r; [|lia..].
+        f_equal. lia.
+  Qed.
+
+  Lemma frame_f_locs_update' fr fr' vs1 vs_new vs_old vs2 val_idxs val_localidxs :
+    val_idxs = seq (length vs1) (length vs_old) ->
+    val_localidxs = map prelude.W.Mk_localidx val_idxs ->
+    frame_rel (λ i, i ∉ val_idxs) fr fr' ->
+    Forall2 (λ i v, f_locs fr' !! localimm i = Some v) val_localidxs vs_new ->
+    f_locs fr  = vs1 ++ vs_old ++ vs2 ->
+    f_locs fr' = vs1 ++ vs_new ++ vs2.
+  Proof.
+    intros Hval_idxs Hval_localidxs Hframe_rel HF Hfr.
+    eapply frame_f_locs_update; eauto.
+    subst val_localidxs.
+    rewrite Forall2_fmap_l in HF.
+    eapply Forall2_impl; [exact HF|].
+    done.
+  Qed.
+
+  Lemma frame_rel_Forall2_update fr fr' vs (val_idxs1 val_idxs2 : list nat) :
+    frame_rel (λ i, i ∉ val_idxs1) fr fr' ->
+    Forall (λ i, i ∉ val_idxs1) val_idxs2 ->
+    Forall2 (λ i v, f_locs fr !! i = Some v) val_idxs2 vs ->
+    Forall2 (λ i v, f_locs fr' !! i = Some v) val_idxs2 vs.
+  Proof.
+    intros [Hmask _] Hdisjoint Hforall.
+    induction Hforall as [| i v idxs vs Hi Hrest IH].
+    - constructor.
+    - apply Forall_cons in Hdisjoint as [Hnotin Hdisjoint].
+      constructor.
+      + rewrite <- Hmask; last exact Hnotin.
+        exact Hi.
+      + exact (IH Hdisjoint).
+  Qed.
+
+  Lemma frame_rel_Forall2_update' fr fr' vs val_localidxs2 (val_idxs1 val_idxs2 : list nat) :
+    val_localidxs2 = map prelude.W.Mk_localidx val_idxs2 ->
+    frame_rel (λ i, i ∉ val_idxs1) fr fr' ->
+    Forall (λ i, i ∉ val_idxs1) val_idxs2 ->
+    Forall2 (λ i v, f_locs fr !! localimm i = Some v) val_localidxs2 vs ->
+    Forall2 (λ i v, f_locs fr' !! localimm i = Some v) val_localidxs2 vs.
+  Proof.
+    intros -> Hfrel Hdisjoint Hforall.
+    rewrite Forall2_fmap_l in Hforall.
+    rewrite Forall2_fmap_l.
+    eapply Forall2_impl.
+    2: {
+      intros x y Hxy.
+      simpl.
+      apply Hxy.
+    }
+    eapply frame_rel_Forall2_update; try done.
+  Qed.
+
+  Lemma value_interp_ref_sz se κ μ τ os :
+    value_interp rti sr se (RefT κ μ τ) (SAtoms os) -∗ ⌜length os = 1⌝.
+  Proof.
+    iIntros "(%sκ & _ & _ & H)".
+    destruct μ.
+    - destruct (lookup_mem se n) eqn:Hn; cbn in Hn.
+      + cbn. rewrite Hn. destruct b.
+        * iDestruct "H" as "(% & % & % & %Hos & _)". by inversion Hos.
+        * iDestruct "H" as "(% & % & %Hos & _)". by inversion Hos.
+      + cbn. by rewrite Hn.
+    - cbn. destruct b.
+      + iDestruct "H" as "(% & % & % & %Hos & _)". by inversion Hos.
+      + iDestruct "H" as "(% & % & %Hos & _)". by inversion Hos.
+  Qed.
+
+  (* useful lemma for proving compat lemmas for instructions erased by the compiler. *)
+  Lemma sem_type_erased M F L WT WL lmask ψ τs1 τs2 :
+    ψ = InstrT τs1 τs2 ->
+    ⊢ (∀ se vs,
+          values_interp rti sr se τs1 vs -∗
+          values_interp rti sr se τs2 vs) -∗
+      have_instr_type_sem rti sr mr M F L WT WL lmask [] ψ L.
+  Proof.
+    iIntros (->) "Hcast".
+    iIntros (se inst lh Henv fr rvs vs θ) "@@@@@@@@@@@@".
+    rewrite app_nil_r.
+    iApply (cwp_val with "[$] [$]"); first done.
+    iFrame.
+    iSplit.
+    - unfold frame_rel.
+      iPureIntro; split.
+      + unfold mask_locs_eq; eauto.
+      + eauto.
+    - by iApply "Hcast".
+  Qed.
+
+  Lemma sem_type_erased_nop M F L WT WL lmask ψ τs1 τs2 :
+    ψ = InstrT τs1 τs2 ->
+    ⊢ (∀ se fr B R os,
+     "%Hse" ∷ ⌜sem_env_interp F se⌝ -∗
+     "#Hinst" ∷ instance_interp rti sr mr M WT (f_inst fr) -∗
+     "#Hlabels"
+     ∷ labels_interp rti sr se (typing.fc_locals F) fr WL lmask 
+         (fc_labels F) B -∗
+     "#Hreturn" ∷ return_interp rti sr se (fc_return F) R -∗
+          values_interp rti sr se τs1 os -∗
+          ▷values_interp rti sr se τs2 os) -∗
+      have_instr_type_sem rti sr mr M F L WT WL lmask [BI_nop] ψ L.
+  Proof.
+    iIntros (->) "Hcast".
+    iIntros (se inst lh fr rvs vs θ Henv) "@@@@@@@@@@@@".
+    iApply cwp_val_app; first done.
+    iApply (cwp_nop with "[$] [$]").
+    iFrame.
+    iSplit.
+    - unfold frame_rel, mask_locs_eq; eauto.
+    - rewrite app_nil_r.
+      iFrame.
+      by iApply "Hcast".
+  Qed.
+
+
+  Lemma has_prim_has_arep η v :
+    has_prim η v ->
+    has_arep (prim_to_arep η) (value_to_atom v).
+  Proof.
+    intros Hprim.
+    destruct v, η; simpl; done.
+  Qed.
+
+  Lemma has_prims_has_areps ηs vs :
+    has_prims ηs vs ->
+    has_areps (map prim_to_arep ηs) (SAtoms (values_to_atoms vs)).
+  Proof.
+    revert ηs.
+    induction vs; intros ηs Hprims.
+    - inversion Hprims; subst.
+      simpl.
+      eexists.
+      by split.
+    - destruct ηs as [| η ηs]; first inversion Hprims.
+      simpl.
+      apply has_areps_cons.
+      apply Forall2_cons in Hprims as [Hprim Hprims].
+      split; first by apply IHvs.
+      by apply has_prim_has_arep.
+  Qed.
+
+  Lemma values_to_atoms_norefs vs :
+    Forall (forall_ptr_atom norefs_ptr_interp) (values_to_atoms vs).
+  Proof.
+    induction vs as [|v vs]; simpl; first done.
+    apply Forall_cons.
+    split.
+    - by destruct v.
+    - apply IHvs.
+  Qed.
+
+  Lemma locals_interp_lookup se L oss i τ_old :
+    L !! i = Some τ_old →
+    locals_interp rti sr se L oss -∗
+    ∃ oss_pre os_mid oss_post,
+    ⌜oss = oss_pre ++ [os_mid] ++ oss_post⌝ ∗
+    locals_interp rti sr se (take i L) oss_pre ∗
+    value_interp rti sr se τ_old (SAtoms os_mid) ∗
+    locals_interp rti sr se (drop (S i) L) oss_post.
+  Proof.
+    iIntros (Hlookup_L) "Hval".
+    iDestruct (big_sepL2_length with "Hval") as %Hoss_len.
+    have Hlookup_oss_i : ∃ os_mid, oss !! i = Some os_mid.
+    {
+      apply lookup_lt_is_Some_2.
+      rewrite -Hoss_len.
+      by eapply lookup_lt_Some.
+    }
+    destruct Hlookup_oss_i as [os_mid Hlookup_oss_i].
+    iExists (take i oss), os_mid, (drop (S i) oss).
+    iSplit.
+    { iPureIntro. symmetry. apply take_drop_middle. exact Hlookup_oss_i. }
+    (* unfold locals_interp. *)
+    have Hsplit_L := take_drop_middle L i τ_old Hlookup_L.
+    have Hsplit_oss := take_drop_middle oss i os_mid Hlookup_oss_i.
+    rewrite <- Hsplit_L, <- Hsplit_oss.
+    iDestruct (big_sepL2_app_inv with "Hval") as "[Hval_pre Hval_rest]".
+    { left. rewrite !length_take. lia. }
+    rewrite Hsplit_L Hsplit_oss.
+    iDestruct "Hval_rest" as "[Hval_mid Hval_post]".
+    unfold locals_interp.
+    iFrame.
+  Qed.
+
+  Lemma locals_interp_length se L oss :
+    locals_interp rti sr se L oss -∗ ⌜length L = length oss⌝.
+  Proof.
+    iIntros "Hval".
+    unfold locals_interp.
+    iDestruct (big_sepL2_length with "Hval") as %Hlen.
+    iPureIntro. exact Hlen.
+  Qed.
+
+  Lemma frame_interp_update_frame se ηss L wl1 wl2 wl vs_idxs vs_wl fr fr' :
+    vs_idxs = seq ((length $ concat ηss) + length wl1) (length wl) ->
+    Forall2 (λ i v, f_locs fr' !! i = Some v) vs_idxs vs_wl ->
+    result_type_interp wl vs_wl ->
+    frame_rel (λ i, i ∉ vs_idxs) fr fr' ->
+    frame_interp rti sr se ηss L (wl1 ++ wl ++ wl2) fr -∗
+    frame_interp rti sr se ηss L (wl1 ++ wl ++ wl2) fr'.
+  Proof.
+    intros Hvs_idxs_wl Hnew_vals Hres Hfrel.
+    iIntros "Hframe".
+    iDestruct "Hframe" as
+      "(%oss & %vss_L & %vs_WL_old & %Hfr & %Hprims & %Hresult & Hatom & Hval)".
+    apply result_type_interp_split in Hresult.
+    destruct Hresult as [vs_wl1 [vs_rest [-> [Hvs_wl1 Hresult]]]].
+    apply result_type_interp_split in Hresult.
+    destruct Hresult as [vs_wl' [vs_wl2 [-> [Hvs_wl' Hvs_wl2]]]].
+    iFrame.
+    iExists (vs_wl1 ++ vs_wl ++ vs_wl2).
+    iPureIntro; split; last split.
+    - rewrite app_assoc.
+      eapply (frame_f_locs_update); [ | done | done | by rewrite -app_assoc].
+      rewrite length_app.
+      apply Forall2_length in Hvs_wl' as <-.
+      apply Forall2_length in Hvs_wl1 as <-.
+      apply Forall2_concat in Hprims.
+      apply Forall2_length in Hprims as <-.
+      done.
+    - done.
+    - apply result_type_interp_combine; first done.
+      by apply result_type_interp_combine; last done.
+  Qed.
+
+  Lemma frame_interp_update_frame' se ηss L wl1 wl2 wl vs_localidxs vs_idxs vs_wl fr fr' :
+    vs_idxs = seq ((length $ concat ηss) + length wl1) (length wl) ->
+    vs_localidxs = map prelude.W.Mk_localidx vs_idxs ->
+    Forall2 (λ i v, f_locs fr' !! localimm i = Some v) vs_localidxs vs_wl ->
+    result_type_interp wl vs_wl ->
+    frame_rel (λ i, i ∉ vs_idxs) fr fr' ->
+    frame_interp rti sr se ηss L (wl1 ++ wl ++ wl2) fr -∗
+    frame_interp rti sr se ηss L (wl1 ++ wl ++ wl2) fr'.
+  Proof.
+    iIntros (Hvs_idxs Hvs_localidxs HF Hres Hframe_rel) "Hfr".
+    iApply frame_interp_update_frame; eauto.
+    subst vs_localidxs.
+    rewrite Forall2_fmap_l in HF.
+    eapply Forall2_impl; [exact HF|].
+    done.
+  Qed.
+
+  Lemma frame_interp_locals_ctx_length se ηss L WL fr :
+    frame_interp rti sr se ηss L WL fr -∗ ⌜length ηss = length L⌝.
+  Proof.
+    iIntros "Hframe".
+    iDestruct "Hframe" as (oss vss_L vs_WL Hf_locs Hhas_prims Hresult) "[Hatom Hval]".
+    iDestruct (locals_interp_length with "Hval") as "->".
+    iDestruct (big_sepL2_length with "Hatom") as "%Hoss_len".
+    iPureIntro.
+    apply Forall2_length in Hhas_prims as ->.
+    done.
+  Qed.
+
+  Lemma frame_interp_update_frame_label se τ_old ηs L wl vs_l vs_idxs os fe fr fr' i τ :
+    let L' := <[i:=τ]> L in
+    L !! i = Some τ_old ->
+    wl_interp (fe_wlocal_offset fe) wl fr ->
+    fe_locals fe !! i = Some ηs ->
+    vs_idxs = seq (sum_list_with length (take i (fe_locals fe))) (length ηs) ->
+    has_prims ηs vs_l ->
+    Forall2 (λ j v, f_locs fr' !! j = Some v) vs_idxs vs_l ->
+    frame_rel (λ j, j ∉ vs_idxs) fr fr' ->
+    atoms_interp os vs_l -∗
+    value_interp rti sr se τ (SAtoms os) -∗
+    frame_interp rti sr se (fe_locals fe) L wl fr -∗
+    frame_interp rti sr se (fe_locals fe) L' wl fr'.
+  Proof.
+    intros L' Hlookup_L Hwl_interp Hlookup Hvs_idxs Hhas_prims_new Hf2 Hfrel.
+    iIntros "Hatoms_new Hvalues Hframe".
+
+    iDestruct (frame_interp_locals_ctx_length with "Hframe") as "%HL_len".
+
+    iDestruct "Hframe" as
+      "(%oss & %vss_L & %vs_WL & %Hfr & %Hhas_prims & %Hresult & Hatoms & Hval)".
+    iFrame (Hresult).
+
+    have Hsplit := take_drop_middle (fe_locals fe) i ηs Hlookup.
+    rewrite <- Hsplit in Hhas_prims.
+    apply List.Forall2_app_inv_l in Hhas_prims as (vss_L_pre & vss_L_rest & Hpre & Hrest & ->).
+    destruct vss_L_rest as [| vs_mid vss_L_post]; [inversion Hrest |].
+    apply Forall2_cons_1 in Hrest as [Hmid Hpost].
+
+    iDestruct (locals_interp_lookup _ _ _ _ _ Hlookup_L with "Hval") as (oss_pre os_mid oss_post Hoss_eq) "[Hval_pre [_ Hval_post]]".
+
+    iEval (rewrite Hoss_eq) in "Hatoms".
+    iDestruct (locals_interp_length with "Hval_pre") as %Hlen_pre.
+    iDestruct (locals_interp_length with "Hval_post") as %Hlen_post.
+    apply Forall2_length in Hpre as Hvs_pre_len.
+    apply Forall2_length in Hmid as Hvs_mid_len.
+    apply Forall2_length in Hpost as Hvs_post_len.
+
+    have Hlen_oss_pre : length oss_pre = length vss_L_pre.
+    { rewrite <- Hlen_pre, length_take, <- Hvs_pre_len, length_take. lia. }
+    have Hlen_oss_post : length oss_post = length vss_L_post.
+    { rewrite <- Hlen_post, length_drop, <- Hvs_post_len, length_drop. lia. }
+
+    iDestruct (big_sepL2_app_inv _ _ _ _ _ with "Hatoms") as "[Hatoms_pre Hatoms_rest]"; first by left.
+    (* NOTE: the atoms_interp for the middle is being thrown away, since the values are being overwritten *)
+    iDestruct (big_sepL2_cons with "Hatoms_rest") as "[_ Hatoms_post]".
+
+    iExists (oss_pre ++ [os] ++ oss_post), (vss_L_pre ++ [vs_l] ++ vss_L_post).
+    iSplit.
+    {
+      iPureIntro.
+      rewrite !concat_app.
+      rewrite concat_app concat_cons in Hfr.
+      rewrite -!app_assoc.
+      rewrite -!app_assoc in Hfr.
+      clear_nils.
+      eapply frame_f_locs_update.
+      4: apply Hfr.
+      3: done.
+      2: done.
+      subst vs_idxs.
+      f_equal; last done.
+      rewrite -sum_list_with_length_concat.
+      eapply Forall2_sum_list_with_length.
+      eapply Forall2_impl; [exact Hpre |].
+      intros ηs' vs' Hprims'.
+      apply Forall2_length in Hprims'.
+      done.
+    }
+    iSplit.
+    {
+      iPureIntro.
+      rewrite <- (take_drop_middle (fe_locals fe) i ηs Hlookup).
+      apply Forall2_app; [exact Hpre |].
+      apply Forall2_cons; by split.
+    }
+    iSplitL "Hatoms_new Hatoms_pre Hatoms_post".
+    - by iFrame.
+    - unfold locals_interp, L'.
+      rewrite insert_take_drop.
+      2: { eapply lookup_lt_Some. exact Hlookup_L. }
+      iApply (big_sepL2_app with "Hval_pre").
+      iApply big_sepL2_cons.
+      iFrame.
+  Qed.
+
+  Lemma frame_interp_update_frame_label' se τ_old ηs L wl vs_l vs_idxs vs_localidxs os fe fr fr' i τ :
+    let L' := <[i:=τ]> L in
+    L !! i = Some τ_old ->
+    wl_interp (fe_wlocal_offset fe) wl fr ->
+    fe_locals fe !! i = Some ηs ->
+    vs_idxs = seq (sum_list_with length (take i (fe_locals fe))) (length ηs) ->
+    vs_localidxs = map prelude.W.Mk_localidx vs_idxs ->
+    has_prims ηs vs_l ->
+    Forall2 (λ j v, f_locs fr' !! localimm j = Some v) vs_localidxs vs_l ->
+    frame_rel (λ j, j ∉ vs_idxs) fr fr' ->
+    atoms_interp os vs_l -∗
+    value_interp rti sr se τ (SAtoms os) -∗
+    frame_interp rti sr se (fe_locals fe) L wl fr -∗
+    frame_interp rti sr se (fe_locals fe) L' wl fr'.
+  Proof.
+    intros L' HlookupL Hwl_interp Hlookup Hvs_idxs Hvs_localidxs Hhas_prims_new Hf2 Hfrel.
+    iIntros "Hatoms Hvalues Hframe".
+    iApply (frame_interp_update_frame_label with "[$] [$] [$]" ); eauto.
+    subst vs_localidxs.
+    rewrite Forall2_fmap_l in Hf2.
+    eapply Forall2_impl; [exact Hf2|].
+    done.
+  Qed.
+
+  Lemma atom_interp_value_type_interp (ι : atomic_rep) (o : atom) (v : value) :
+    has_arep ι o →
+    atom_interp o v -∗
+    ⌜value_type_interp (translate_arep ι) v⌝.
+  Proof.
+    intros Harep.
+    destruct ι, o; simpl in *; try done.
+    {
+      iIntros "(%n & %n32 & %Hrep & -> & _)".
+      iExists _; eauto.
+    }
+    all: iIntros "->"; iPureIntro; exists n; done.
+  Qed.
+
+  Lemma result_type_interp_of_atoms_interp ιs os vs :
+    has_areps ιs (SAtoms os) ->
+    atoms_interp os vs -∗
+    ⌜result_type_interp (map translate_arep ιs) vs⌝.
+  Proof.
+    revert os vs.
+    induction ιs as [| ι ιs' IH]; intros os vs Hιs'.
+    - (* ιs = [] *)
+      destruct Hιs' as (os' & Heq & Hfa).
+      inversion Heq; subst.
+      inversion Hfa; subst.
+      iIntros "Hinterp".
+      iDestruct (atoms_interp_nil_l with "Hinterp") as "->".
+      iPureIntro.
+      constructor.
+    - (* ιs = ι :: ιs' *)
+      destruct os as [| o os].
+      {
+        destruct Hιs' as (os' & Heq & Hfa).
+        inversion Heq; subst.
+        inversion Hfa.
+      }
+      apply has_areps_cons in Hιs' as [Hιs'_tl Hιs'_hd].
+      iIntros "Hinterp".
+      iDestruct (atoms_interp_cons_l with "Hinterp") as
+      "(%v & %vs' & -> & Hv & Hos)".
+      iDestruct (IH _ _ Hιs'_tl with "Hos") as "%Htl".
+      iDestruct (atom_interp_value_type_interp ι o v Hιs'_hd with "Hv") as "%Hhd".
+      iPureIntro.
+      simpl.
+      by constructor.
+  Qed.
+
+  Lemma value_type_interp_of_default ty :
+    value_type_interp ty (default_of_value_type ty).
+  Proof. destruct ty; by eexists. Qed.
+
+  Lemma result_type_interp_of_defaults tys :
+    result_type_interp tys (default_of_value_types tys).
+  Proof.
+    induction tys as [| ty tys IH].
+    - constructor.
+    - constructor; last done.
+      apply value_type_interp_of_default.
+  Qed.
+
+  Lemma empty_closure_interp se ϕ cl :
+    closure_interp rti sr ϕ senv_empty cl -∗
+    closure_interp rti sr ϕ se cl.
+  Proof.
+    (* This seems true? *)
+    iIntros "H".
+    cbn.
+  Admitted.
+
+
+  Lemma skind_rec_interp_unfold sκ T (se: semantic_env (Σ:=Σ)) sv :
+    skind_rec_interp sκ T se sv ≡ (▷ T (senv_insert_type sκ (skind_rec_interp sκ T se) se) sv)%I.
+  Proof.
+    simpl.
+    set f := (λ T0 : leibnizO semantic_value -n> iPropO Σ, λne sv0 : leibnizO semantic_value, (▷ T (se.1, (sκ, T0) :: se.2) sv0)%I).
+     etransitivity.
+     - exact (fixpoint_unfold f sv).
+     - simpl. reflexivity.
+  Qed.
+
+  Lemma rec_interp_unfold κ T (se: semantic_env (Σ:=Σ)) sv :
+    rec_interp κ T se sv ≡
+    match eval_kind_se se κ with
+    | Some sκ => ▷ T (senv_insert_type sκ (skind_rec_interp sκ T se) se) sv
+    | None => False
+    end%I.
+  Proof.
+    unfold rec_interp. simpl.
+    destruct (eval_kind se κ) as [sκ|]; simpl.
+    - set f := (λ T0 : leibnizO semantic_value -n> iPropO Σ,
+      λne sv0 : leibnizO semantic_value,
+      (▷ T (se.1, (sκ, T0) :: se.2) sv0)%I).
+      etransitivity.
+      + exact (fixpoint_unfold f sv).
+      + simpl. reflexivity.
+    - reflexivity.
+  Qed.
+
+  Lemma value_interp_type_plug se vs ηs :
+    ⌜has_prims ηs vs⌝ -∗
+    value_interp rti sr se (type_plug_prim ηs) (SAtoms (values_to_atoms vs)).
+  Proof.
+    iIntros "%Hprims".
+    rewrite value_interp_eq /add_skind_interp.
+    unfold type_plug_prim, type_plug. simpl.
+    set ρ := ProdR (map (AtomR ∘ prim_to_arep) ηs).
+    have Heval : eval_rep se ρ = Some (map prim_to_arep ηs).
+    { apply eval_rep_prod_atoms. }
+    iExists (SVALTYPE (map prim_to_arep ηs) NoRefs).
+    iSplit.
+    - iPureIntro. unfold type_skind. simpl.
+      have Heval_kind := eval_kind_of_eval_rep se ρ _ Heval NoRefs.
+      rewrite -Heval_kind.
+      done.
+    - apply has_prims_has_areps in Hprims as Hareps.
+      iSplit.
+      + iPureIntro. simpl.
+        split; first done.
+        apply values_to_atoms_norefs.
+      + iExists (map prim_to_arep ηs).
+        iSplit; [iPureIntro; exact Heval |].
+        done.
+  Qed.
+
+  Lemma type_interp_skind_svalue (τ : type) se sv :
+    type_interp rti sr τ se sv -∗ ∃ sκ, ⌜type_skind se τ = Some sκ⌝ ∗ ⌜skind_has_svalue sκ sv⌝.
+  Proof.
+    iIntros "H".
+    rewrite type_interp_eq.
+    iDestruct "H" as (sκ) "[%Hsk [%Hsv _]]".
+    iExists sκ. by iSplit; iPureIntro.
+  Qed.
+
+  (* TODO: might need to change. @Elan *)
+  Lemma fold_type_interp_subst (se : semantic_env (Σ:=Σ)) (τ : type) (κ : kind) sκ sv :
+    eval_kind se κ = Some sκ →
+    type_interp rti sr (subst_type VarM VarR VarS (unscoped.scons (RecT κ τ) VarT) τ) se sv ⊣⊢
+    type_interp rti sr τ (senv_insert_type sκ (skind_rec_interp sκ (type_interp rti sr τ) se) se) sv.
+  Proof. Admitted.
+
+  (* This is actually 100% proved in inst.v under ..._COPY_STUPID *)
+  (* so if this can be used instead of the one above that's cool *)
+  (* idk if it can be though *)
+  (* bc using it requires proving values_interp == skind_rec_interp sk type_interp ... *)
+  (* which the previous version of the proof *almost* proved except for the svalue_has_skind thingy *)
+  (* so maybe it's possible... *)
+  Lemma fold_type_interp_subst_TEST (se : semantic_env (Σ:=Σ)) F (τ : type) (κ : kind) sκ sv :
+    sem_env_interp F se ->
+    has_kind F (RecT κ τ) κ ->
+    eval_kind se κ = Some sκ →
+    type_interp rti sr τ (senv_insert_type sκ (value_interp rti sr se (RecT κ τ)) se) sv ⊣⊢
+    type_interp rti sr (subst_type VarM VarR VarS (unscoped.scons (RecT κ τ) VarT) τ) se sv.
+  Proof.
+  Admitted.
+
+  Lemma fold_type_interp_TEST (se : semantic_env (Σ:=Σ)) F (τ : type) (κ : kind) sκ sv :
+    sem_env_interp F se ->
+    has_kind F (RecT κ τ) κ -> (* both these above are tests *)
+    eval_kind se κ = Some sκ →
+    type_interp rti sr (RecT κ τ) se sv ⊣⊢
+    ⌜skind_has_svalue sκ sv⌝ ∗
+    ▷ type_interp rti sr (subst_type VarM VarR VarS (unscoped.scons (RecT κ τ) VarT) τ) se sv.
+  Proof.
+    intros Hse Hkind Hκ.
+    iSplit.
+    - iIntros "H".
+      iEval (rewrite type_interp_eq) in "H".
+      iDestruct "H" as "(%sκ' & %Hκ' & %Hsv & Hrec)".
+      unfold type_skind in Hκ'. simpl in Hκ'.
+      rewrite Hκ in Hκ'. simplify_eq.
+      iSplit; first done.
+
+
+      iAssert ((skind_rec_interp sκ' (type_interp rti sr τ) se ≡ value_interp rti sr se (RecT κ τ)
+                  )%I) as "#TheEquiv". {
+        admit. (* most of this is in inst in fold_type_interp_subst_COPY *)
+        (* note that I'm pretty sure it's true. There's a weird part with type_skind in
+           a new environment. But I *think* it's okay. Hopefully. Idk maybe not.
+           but if this is true (and if we can get the rewrites below to work) then this whole
+           thing is proven
+         *)
+      }
+
+
+      iEval (cbn [pre_type_interp]) in "Hrec".
+      iEval (rewrite (rec_interp_unfold κ (type_interp rti sr τ) se sv)) in "Hrec".
+      replace (eval_kind_se se κ) with (eval_kind se κ); last done.
+      iEval (rewrite Hκ) in "Hrec".
+
+      Fail iRewrite "TheEquiv". (* I'm pissed *)
+      iAssert ((▷ type_interp rti sr τ
+               (senv_insert_type sκ' (value_interp rti sr se (RecT κ τ)) se) sv)%I)
+        with "[Hrec]" as "Hrec". {
+        (* okay whatever, use TheEquiv *)
+        admit.
+      }
+      iEval (rewrite <- (fold_type_interp_subst_TEST se F τ κ sκ' sv Hse Hkind Hκ)).
+      iExact "Hrec".
+    - iIntros "[%Hsv Hτrec]".
+      iEval (rewrite type_interp_eq).
+      iExists sκ.
+      iSplit. { iPureIntro. unfold type_skind. simpl. by rewrite Hκ. }
+      iSplit. { iPureIntro. exact Hsv. }
+
+
+      iAssert ((skind_rec_interp sκ (type_interp rti sr τ) se ≡ value_interp rti sr se (RecT κ τ)
+                  )%I) as "#TheEquiv". {
+        admit. (* most of this is in inst, as above *)
+      }
+
+
+      iEval (cbn [pre_type_interp]).
+      iEval (rewrite (rec_interp_unfold κ (type_interp rti sr τ) se sv)).
+      replace (eval_kind_se se κ) with (eval_kind se κ); last done.
+      iEval (rewrite Hκ).
+      iEval (rewrite <- (fold_type_interp_subst_TEST se F τ κ sκ sv Hse Hkind Hκ)) in "Hτrec".
+
+      Fail iRewrite "TheEquiv". (* of course but just do that *)
+
+      (*iExact "Hτrec".*)
+  Admitted.
+  Lemma fold_type_interp (se : semantic_env (Σ:=Σ)) (τ : type) (κ : kind) sκ sv :
+    eval_kind se κ = Some sκ →
+    type_interp rti sr (RecT κ τ) se sv ⊣⊢
+    ⌜skind_has_svalue sκ sv⌝ ∗
+    ▷ type_interp rti sr (subst_type VarM VarR VarS (unscoped.scons (RecT κ τ) VarT) τ) se sv.
+  Proof.
+  Admitted.
+End properties.
